thesis

Examples.v
@@ -30,6 +30,175 @@ Proof.
   try (destruct (decrypt (encrypt _ m k) k'); [inversion p; apply is_dec_info in H1; assumption | exfalso; rewrite <- hh in H0; rewrite <- hh in H; apply (notBadContra m k k' H H0 i)]).
 Qed.
 
+
+(* Simple increment example *)
+
+Definition incPayload (m:message Basic) : (message Basic) :=
+  match m with
+  | basic n => basic (n + 1)
+  | _ => bad Basic                 
+  end.
+
+Definition proto1A (m:(message Basic)) :=
+  send m;
+  x <- receive;
+  ReturnC (t:=Basic) x.
+Check proto1A.
+
+Definition proto1B :=
+  x <- receive;
+  send (incPayload x);
+  ReturnC x.
+Check proto1B.
+
+Theorem dual1AB : forall (x:message Basic), Dual (proto1A x) proto1B.
+Proof.
+  cbv.
+  split.
+  reflexivity.
+  split.
+    reflexivity.
+    trivial.
+Qed.
+
+Theorem incPropertyAB : forall x x' st st',
+    multi st _ _ _ (proto1A x) proto1B (ReturnC x') st' ->
+    x' = incPayload x.
+Proof.
+  intros x x' st st' multiProof.
+  dep_destruct multiProof. clear multiProof.
+  dep_destruct s0. dep_destruct s1. clear s0. clear s1.
+  dep_destruct x2. clear x2.
+  dep_destruct s0. dep_destruct s1. clear s0. clear s1.
+  dep_destruct x3. reflexivity.
+  inversion s1.
+Qed.
+
+
+(* Needham Schroeder *)
+
+
+Definition aNonceSecret := 11.
+Definition bNonceSecret := 22.
+Definition aNonce := (basic aNonceSecret).
+Definition bNonce := (basic bNonceSecret).
+
+Definition aPub := (public 1).
+Definition bPub := (public 2).
+Definition aPubBad := (public 3).
+Definition bPubBad := (public 4).
+Definition aPri := (private 1).
+Definition bPri := (private 2).
+Definition aPriBad := (private 5).
+Definition bPriBad := (private 6).
+ 
+
+Definition Needham_A (myPri theirPub:keyType) :=
+  send (encrypt _ aNonce theirPub);
+  x <- receive; (* x : Encrypt (Pair Basic Basic) *) 
+  let y : (message (Pair Basic Basic)):= decryptM x myPri in (* y : Pair Basic Basic *)
+  let y' := (pairFst y) in
+  let y'' := (pairSnd y) in 
+  send (encrypt _ y'' theirPub);
+  ReturnC (pair _ _ y' y''). Check Needham_A.
+
+Definition Needham_B (myPri theirPub:keyType) :=
+  ReceiveC (fun x: message (Encrypt Basic) => ( 
+  (*x <- receive; (* x : Encrypt Basic *) *)
+  let y : (message Basic) := decryptM x myPri in (* y : Basic *)
+  send (encrypt (Pair Basic Basic) (pair _ _ y bNonce) theirPub);
+  ReceiveC (fun z : message (Encrypt Basic) => ( 
+  (*z <- receive; (* z : Encrypt Basic *) *)
+                let z' := decryptM z myPri in   (* z' : Basic *)
+  (*ReturnC y)))).  Check Needham_B. *)
+  ReturnC (pair _ _ y z'))))). Check Needham_B.
+
+Example dualNeedham : forall ka ka' kb kb',
+    Dual (Needham_A ka kb') (Needham_B kb ka').
+Proof.
+  intros.
+  split. reflexivity.
+  split. reflexivity.
+  split. reflexivity.
+  reflexivity.
+Qed.
+
+Theorem needham_A_auth : forall (k:keyType) (x:message Basic) st st', 
+    multi
+      st
+      _ _ _
+      (Needham_A k bPub)
+      (Needham_B bPri aPub)
+      (ReturnC (pair _ _ x bNonce))
+      st'
+    -> (k = inverse aPub).
+Proof.
+  intros k x st st' multiProof.
+  dep_destruct multiProof. clear multiProof.
+  dep_destruct s0. dep_destruct s1. clear s0. clear s1.
+  dep_destruct x2. clear x2.
+  dep_destruct s0. dep_destruct s1. clear s0. clear s1.
+  dep_destruct x3. clear x3.
+  dep_destruct s1. dep_destruct s4. clear s1. clear s4.
+  dep_destruct x2. clear x2. clear x. cbn in x0.
+  unfold decryptM in x0.
+  destruct  (decrypt
+            (encrypt _ (pair _ _ aNonce (basic bNonceSecret)) aPub)
+            k) as [p | _].
+  destruct p as (m , i).
+    dep_destruct i. reflexivity. simpl in x0.
+    inversion x0.
+  inversion s4.
+Qed.
+
+
+Definition normalizeState : State -> State := fun _ => emptyState.
+
+(* Future Work *)
+Definition hoare_triple{p1t p2t p3t:protoType}{t:type}
+           (P:Assertion)
+           (p1:protoExp p1t) (p2:protoExp p2t) (p3:protoExp p3t)
+           (Q:Assertion) : Prop :=
+  forall st st',
+     P st ->
+     multi st _ _ _ p1 p2 p3 st' ->
+     Q (normalizeState st').
+
+Definition notInPb : (message Basic) -> State -> Prop := fun _ _ => True.
+Definition inPb : (message Basic) -> State -> Prop := fun _ _ => True.
+
+
+Definition learnedB {p1t p2t p3t:protoType}
+           (m:message Basic)
+           (p1:protoExp p1t) (p2:protoExp p2t) (p3:protoExp p3t) : Prop :=
+  hoare_triple (t:=Basic) (notInPb m) p1 p2 p3 (inPb m).
+ 
+
+Definition p1 :=
+  send (basic 33);
+  EpsC.
+
+Definition p2 :=
+  x <- receive;
+  ReturnC (t:=Basic) x.
+
+Definition learnedProof : learnedB (basic 33) p2 p1 (ReturnC (basic 33)).
+Proof.
+  intros.
+  unfold p1. unfold p2. unfold learnedB. unfold hoare_triple.
+  intros.
+  dep_destruct H0. clear H0.
+  dep_destruct s0. dep_destruct s1. clear s0. clear s1.
+  dep_destruct x1. clear x1. simpl. cbn. trivial.
+  Abort.
+
+
+
+
+
+
+
+
 (* Simplest possible encrypt/decrypt protocol pair *)
 Definition protoEncrypt1 (theirPub:keyType) :=
   send (encrypt _ (basic 42) theirPub);
@@ -89,243 +258,6 @@ Proof.
   assumption.
   inversion s2.
 Qed.
-
-
-
-
-
-(* Needham Schroeder *)
-
-
-Definition aNonceSecret := 11.
-Definition bNonceSecret := 22.
-Definition aNonce := (basic aNonceSecret).
-Definition bNonce := (basic bNonceSecret).
-
-Definition aPub := (public 1).
-Definition bPub := (public 2).
-Definition aPubBad := (public 3).
-Definition bPubBad := (public 4).
-Definition aPri := (private 1).
-Definition bPri := (private 2).
-Definition aPriBad := (private 5).
-Definition bPriBad := (private 6).
-
-
-Definition Needham_A (myPri theirPub:keyType) :=
-  send (encrypt _ aNonce theirPub);
-  x <- receive; (* x : Encrypt (Pair Basic Basic) *) 
-  let y := decryptM x myPri in (* y : Pair Basic Basic *)
-  (*let y' := (pairFst (t1:=Basic) (t2:=Basic) y) in *)
-  let y'' := (pairSnd (t1:=Basic) (t2:=Basic) y) in 
-  send (encrypt _ y'' theirPub);
-  ReturnC (y''). Check Needham_A.
-
-Definition Needham_B (myPri theirPub:keyType) :=
-  ReceiveC (fun x: message (Encrypt Basic) => ( 
-  (*x <- receive; (* x : Encrypt Basic *) *)
-  let y : (message Basic) := decryptM x myPri in (* y : Basic *)
-  send (encrypt (Pair Basic Basic) (pair _ _ y bNonce) theirPub);
-  ReceiveC (fun z : message (Encrypt Basic) => ( 
-  (*z <- receive; (* z : Encrypt Basic *) *)
-  let z' := decryptM z myPri in   (* z' : Basic *)
-  ReturnC y)))). Check Needham_B.
-
-Theorem needham_A_auth : forall k st st',
-    multi
-      st
-      _ _ _
-      (Needham_A k bPub)
-      (Needham_B bPri aPub)
-      (ReturnC bNonce)
-      st'
-    -> (k = inverse aPub).
-Proof.
-  intros.
-  dep_destruct H. clear H.
-  dep_destruct s0. dep_destruct s1. clear s0. clear s1.
-  dep_destruct x1. clear x1.
-  dep_destruct s0. dep_destruct s1. clear s0. clear s1.
-  dep_destruct x2. clear x2.
-  dep_destruct s1. dep_destruct s4. clear s1. clear s4.
-  dep_destruct x1. clear x1. clear x. clear x0. cbn in x2.
-    unfold decryptM in x2.
-    destruct  (decrypt
-              (encrypt _ (pair _ _ aNonce (basic bNonceSecret)) aPub)
-              k).
-      destruct p. assumption.
-      inversion x2.
-  
-    inversion s5.
-Qed.
-
-
-Definition incPayload (m:message Basic) : (message Basic) :=
-  match m with
-  | basic n => basic (n + 1)
-  | _ => bad Basic                 
-  end.
-
-Definition proto4 (payload4:(message Basic)) :=
-  send payload4;
-  x <- receive;
-  ReturnC (t:=Basic) x.
-Check proto4.
-
-Definition proto5 :=
-  x <- receive;
-  send (incPayload x);
-  ReturnC x.
-Check proto5.
-
-Example dual45 : forall x, Dual (proto4 x) proto5.
-Proof.
-  cbv.
-  split.
-  reflexivity.
-  split.
-    reflexivity.
-    trivial.
-Qed.
-
-Definition property45 : forall x4 x5 st st',
-    multi st _ _ _ (proto4 x4) proto5 (ReturnC x5) st' ->
-    x5 = incPayload x4.
-Proof.
-  intros.
-  dep_destruct H. clear H.
-  dep_destruct s0. dep_destruct s1. clear s0. clear s1.
-  dep_destruct x1. clear x1.
-  dep_destruct s0. dep_destruct s1. clear s0. clear s1.
-  dep_destruct x2. reflexivity. 
-  inversion s1.
-Qed.
-    
-    
-
-
-Definition hoare_triple{p1t p2t p3t:protoType}{t:type}
-           (P:Assertion)
-           (p1:protoExp p1t) (p2:protoExp p2t) (p3:protoExp p3t)
-           (Q:Assertion) : Prop :=
-  forall st st',
-     P st ->
-     multi st _ _ _ p1 p2 p3 st' ->
-     Q (newState st').
-
-(*Definition inPb : forall mt (m:message mt) (pf: mt = Basic) (s:State),
-    Prop.
-Proof.
-  intros. subst. destruct (my_in m s.(basics)). exact True. exact False.
-Qed.
-
-Definition inPk : forall mt (m:message mt) (pf: mt = Key) (s:State),
-    Prop.
-Proof.
-  intros. subst. destruct (my_in m s.(keys)). exact True. exact False.
-Qed.
-*)
-
-Definition inPb (m:message Basic) (s:State) :=
-  if (my_inB m s.(basics)) then True
-  else False.
-
-Definition inPk (m:message Key) (s:State) :=
-  if (my_inK m s.(keys)) then True
-  else False.
-         
-
-(*Definition inP t (m:message t) (s:State) :=
-  match t as t' return (t = t') -> Prop with
-  | Basic => fun pf => (inPb t m pf s)
-  | Key => fun pf => (inPk t m pf s)
-  | _ => fun _ => False                 
-  end (eq_refl t). 
-
-Definition notInP t (m:message t) (s:State) :=
-  ~ (inP t m s).
- *)
-
-Definition notInPb (m:message Basic) (s:State) :=
-  ~ (inPb m s).
-
-
-
-Definition learnedB {p1t p2t p3t:protoType}
-           (m:message Basic)
-           (p1:protoExp p1t) (p2:protoExp p2t) (p3:protoExp p3t) : Prop :=
-  hoare_triple (t:=Basic) (notInPb m) p1 p2 p3 (inPb m).
- 
-
-Definition p1 :=
-  send (basic 33);
-  EpsC.
-
-Definition p2 :=
-  x <- receive;
-  ReturnC (t:=Basic) x.
-
-Definition learnedProof : learnedB (basic 33) p2 p1 (ReturnC (basic 33)).
-Proof.
-  intros.
-  unfold p1. unfold p2. unfold learnedB. unfold hoare_triple.
-  intros.
-  dep_destruct H0. clear H0.
-  dep_destruct s0. dep_destruct s1. clear s0. clear s1.
-  dep_destruct x1. clear x1. simpl. cbn. trivial.
-  inversion s1.
-Qed.
-
-Definition p3Payload := (basic 42).
-Definition p3 :=
-  send encrypt _ p3Payload (public 0);
-  EpsC.
-
-Definition p4 :=
-  x <- receive;
-  ReturnC (t:=Encrypt Basic) x.
-
-Axiom inInfo : forall (m:message Key) (st:State),
-    inPk m st ->
-    exists kl b kob bob, st = (mkState (m :: kl) b kob bob).
-
-Definition hoare_triple'{p1t p2t p3t:protoType}{t:type} (st:State)
-           (p1:protoExp p1t) (p2:protoExp p2t) (p3:protoExp p3t)
-           (Q:Assertion) : Prop :=
-  forall st',
-     multi st _ _ _ p1 p2 p3 st' ->
-     Q (newState st').
-
-Definition notLearnedIf : hoare_triple' (t:= Encrypt Basic)
-                          emptyState
-                          p4 p3 (ReturnC (encrypt _ p3Payload (public 0)))
-                          (notInPb p3Payload).
-Proof.
-  unfold p3. unfold p4. unfold hoare_triple'.
-  intros.
-  dep_destruct H. clear H. 
-  dep_destruct s0. clear s0. dep_destruct s1. clear s1.
-  cbn in x1. 
-  dep_destruct x1. cbv. intros H. inversion H.
-  inversion s2.
-Qed.
-
-Definition learnedIf : hoare_triple' (t:= Encrypt Basic)
-                       (updateState (key (public 0)) emptyState)
-                       p4 p3 (ReturnC (encrypt _ p3Payload (public 0)))
-                       (inPb p3Payload).
-Proof.
-  unfold p3. unfold p4. unfold hoare_triple'.
-  intros.
-  dep_destruct H. clear H. 
-  dep_destruct s0. clear s0. dep_destruct s1. clear s1.
-  cbn in x1.
-  dep_destruct x1. clear x1. cbv. trivial.
-  inversion s2.
-Qed.
-
-  
-  
   
 
 
